02_FORMAL/coq/properties/NonInterference.v
@@ -10,7 +10,10 @@
 Require Import TERAS.foundations.Syntax.
 Require Import TERAS.foundations.Semantics.
 Require Import TERAS.foundations.Typing.
+Require Import TERAS.type_system.Preservation.
 Require Import Coq.Lists.List.
+Require Import Coq.Logic.FunctionalExtensionality.
+Require Import Coq.Program.Equality.
 Require Import Coq.Strings.String.
 Import ListNotations.
 
@@ -21,6 +24,49 @@ Parameter observer : security_level.
 Definition is_low (l : security_level) : Prop :=
   sec_leq l observer.
 
+(** Closed expressions: no free variables. *)
+Definition closed_expr (e : expr) : Prop :=
+  forall x, ~ free_in x e.
+
+Definition closed_except (x : ident) (e : expr) : Prop :=
+  forall y, y <> x -> ~ free_in y e.
+
+Lemma closed_expr_lam : forall x T body,
+  closed_except x body ->
+  closed_expr (ELam x T body).
+Proof.
+  intros x T body Hclosed y Hfree. simpl in Hfree.
+  destruct Hfree as [Hyneq Hfree].
+  apply (Hclosed y Hyneq) in Hfree. contradiction.
+Qed.
+
+Lemma closed_expr_pair : forall v1 v2,
+  closed_expr v1 ->
+  closed_expr v2 ->
+  closed_expr (EPair v1 v2).
+Proof.
+  intros v1 v2 Hc1 Hc2 y Hfree. simpl in Hfree.
+  destruct Hfree as [Hfree | Hfree].
+  - apply (Hc1 y) in Hfree. contradiction.
+  - apply (Hc2 y) in Hfree. contradiction.
+Qed.
+
+Lemma closed_expr_inl : forall v T,
+  closed_expr v ->
+  closed_expr (EInl v T).
+Proof.
+  intros v T Hc y Hfree. simpl in Hfree.
+  apply (Hc y) in Hfree. contradiction.
+Qed.
+
+Lemma closed_expr_inr : forall v T,
+  closed_expr v ->
+  closed_expr (EInr v T).
+Proof.
+  intros v T Hc y Hfree. simpl in Hfree.
+  apply (Hc y) in Hfree. contradiction.
+Qed.
+
 (** ** Logical Relation
     
     We define a binary logical relation R_V(T) on values.
@@ -28,12 +74,12 @@ Definition is_low (l : security_level) : Prop :=
 *)
 
 Fixpoint val_rel (T : ty) (v1 v2 : expr) {struct T} : Prop :=
-  value v1 /\ value v2 /\
+  value v1 /\ value v2 /\ closed_expr v1 /\ closed_expr v2 /\
   match T with
   | TUnit => v1 = EUnit /\ v2 = EUnit
-  | TBool => v1 = v2
-  | TInt => v1 = v2
-  | TString => v1 = v2
+  | TBool => exists b, v1 = EBool b /\ v2 = EBool b
+  | TInt => exists n, v1 = EInt n /\ v2 = EInt n
+  | TString => exists s, v1 = EString s /\ v2 = EString s
   | TBytes => v1 = v2
   
   | TSecret T' => True
@@ -54,26 +100,828 @@ Fixpoint val_rel (T : ty) (v1 v2 : expr) {struct T} : Prop :=
       forall x y, val_rel T1 x y -> 
         forall st1 st2 ctx,
           exists (v1' : expr) (v2' : expr) (st1' : store) (st2' : store) (ctx' : effect_ctx),
-            (EApp v1 x, st1, ctx) -->* (v1', st1', ctx) /\
-            (EApp v2 y, st2, ctx) -->* (v2', st2', ctx) /\
+            (EApp v1 x, st1, ctx) -->* (v1', st1', ctx') /\
+            (EApp v2 y, st2, ctx) -->* (v2', st2', ctx') /\
             val_rel T2 v1' v2'
 
   | TCapability _ => True
   | TProof _ => True
   end.
 
+Lemma val_rel_closed_left : forall T v1 v2,
+  val_rel T v1 v2 ->
+  closed_expr v1.
+Proof.
+  induction T; simpl; intros v1 v2 Hrel;
+    destruct Hrel as [_ [_ [Hc1 [Hc2 _]]]]; exact Hc1.
+Qed.
+
+Lemma val_rel_closed_right : forall T v1 v2,
+  val_rel T v1 v2 ->
+  closed_expr v2.
+Proof.
+  induction T; simpl; intros v1 v2 Hrel;
+    destruct Hrel as [_ [_ [Hc1 [Hc2 _]]]]; exact Hc2.
+Qed.
+
+Lemma val_rel_value_left : forall T v1 v2,
+  val_rel T v1 v2 ->
+  value v1.
+Proof.
+  induction T; simpl; intros v1 v2 Hrel;
+    destruct Hrel as [Hv1 _]; exact Hv1.
+Qed.
+
+Lemma val_rel_value_right : forall T v1 v2,
+  val_rel T v1 v2 ->
+  value v2.
+Proof.
+  induction T; simpl; intros v1 v2 Hrel;
+    destruct Hrel as [_ [Hv2 _]]; exact Hv2.
+Qed.
+
 (** Expression Relation: Related expressions reduce to related values *)
 Definition exp_rel (T : ty) (e1 e2 : expr) : Prop :=
   forall st1 st2 ctx,
     exists (v1 : expr) (v2 : expr) (st1' : store) (st2' : store) (ctx' : effect_ctx),
-      (e1, st1, ctx) -->* (v1, st1', ctx) /\
-      (e2, st2, ctx) -->* (v2, st2', ctx) /\
+      (e1, st1, ctx) -->* (v1, st1', ctx') /\
+      (e2, st2, ctx) -->* (v2, st2', ctx') /\
       val_rel T v1 v2.
 
 Notation "e1 '~' e2 ':' T" := (exp_rel T e1 e2) (at level 40).
 Notation "v1 '~~' v2 ':' T" := (val_rel T v1 v2) (at level 40).
 
-(** ** Fundamental Theorem (Stub) *)
+(** ** Environment Substitution *)
+
+Definition rho_shadow (rho : ident -> expr) (x : ident) : ident -> expr :=
+  fun y => if String.eqb y x then EVar y else rho y.
+
+Definition rho_extend (rho : ident -> expr) (x : ident) (v : expr) : ident -> expr :=
+  fun y => if String.eqb y x then v else rho y.
+
+Fixpoint subst_rho (rho : ident -> expr) (e : expr) : expr :=
+  match e with
+  | EUnit => EUnit
+  | EBool b => EBool b
+  | EInt n => EInt n
+  | EString s => EString s
+  | EVar x => rho x
+  | ELam x T body => ELam x T (subst_rho (rho_shadow rho x) body)
+  | EApp e1 e2 => EApp (subst_rho rho e1) (subst_rho rho e2)
+  | EPair e1 e2 => EPair (subst_rho rho e1) (subst_rho rho e2)
+  | EFst e1 => EFst (subst_rho rho e1)
+  | ESnd e1 => ESnd (subst_rho rho e1)
+  | EInl e1 T => EInl (subst_rho rho e1) T
+  | EInr e1 T => EInr (subst_rho rho e1) T
+  | ECase e x1 e1 x2 e2 =>
+      ECase (subst_rho rho e)
+            x1 (subst_rho (rho_shadow rho x1) e1)
+            x2 (subst_rho (rho_shadow rho x2) e2)
+  | EIf e1 e2 e3 => EIf (subst_rho rho e1) (subst_rho rho e2) (subst_rho rho e3)
+  | ELet x e1 e2 =>
+      ELet x (subst_rho rho e1) (subst_rho (rho_shadow rho x) e2)
+  | EPerform eff e1 => EPerform eff (subst_rho rho e1)
+  | EHandle e1 x h =>
+      EHandle (subst_rho rho e1) x (subst_rho (rho_shadow rho x) h)
+  | ERef e1 l => ERef (subst_rho rho e1) l
+  | EDeref e1 => EDeref (subst_rho rho e1)
+  | EAssign e1 e2 => EAssign (subst_rho rho e1) (subst_rho rho e2)
+  | EClassify e1 => EClassify (subst_rho rho e1)
+  | EDeclassify e1 e2 => EDeclassify (subst_rho rho e1) (subst_rho rho e2)
+  | EProve e1 => EProve (subst_rho rho e1)
+  | ERequire eff e1 => ERequire eff (subst_rho rho e1)
+  | EGrant eff e1 => EGrant eff (subst_rho rho e1)
+  end.
+
+Lemma free_in_subst_rho : forall x rho e,
+  free_in x (subst_rho rho e) ->
+  exists y, free_in y e /\ free_in x (rho y).
+Proof.
+  intros x rho e.
+  generalize dependent rho.
+  generalize dependent x.
+  induction e; intros x rho Hfree; simpl in Hfree; try contradiction.
+  - exists i. split; simpl; auto.
+  - destruct Hfree as [Hneq Hfree].
+    destruct (IHe x (rho_shadow rho i) Hfree) as [y [Hy Hrho]].
+    assert (y <> i) as Hyneq.
+    { intro Heq. subst.
+      unfold rho_shadow in Hrho. rewrite String.eqb_refl in Hrho. simpl in Hrho.
+      apply Hneq. exact Hrho. }
+    exists y. split.
+    + simpl. split; assumption.
+    + unfold rho_shadow in Hrho.
+      rewrite (proj2 (String.eqb_neq y i) Hyneq) in Hrho. exact Hrho.
+  - destruct Hfree as [Hfree | Hfree].
+    + destruct (IHe1 x rho Hfree) as [y [Hy Hrho]].
+      exists y. split. left. exact Hy. exact Hrho.
+    + destruct (IHe2 x rho Hfree) as [y [Hy Hrho]].
+      exists y. split. right. exact Hy. exact Hrho.
+  - destruct Hfree as [Hfree | Hfree].
+    + destruct (IHe1 x rho Hfree) as [y [Hy Hrho]].
+      exists y. split. left. exact Hy. exact Hrho.
+    + destruct (IHe2 x rho Hfree) as [y [Hy Hrho]].
+      exists y. split. right. exact Hy. exact Hrho.
+  - destruct (IHe x rho Hfree) as [y [Hy Hrho]].
+    exists y. split. exact Hy. exact Hrho.
+  - destruct (IHe x rho Hfree) as [y [Hy Hrho]].
+    exists y. split. exact Hy. exact Hrho.
+  - destruct (IHe x rho Hfree) as [y [Hy Hrho]].
+    exists y. split. exact Hy. exact Hrho.
+  - destruct (IHe x rho Hfree) as [y [Hy Hrho]].
+    exists y. split. exact Hy. exact Hrho.
+  - destruct Hfree as [Hfree | [Hfree | Hfree]].
+    + destruct (IHe1 x rho Hfree) as [y [Hy Hrho]].
+      exists y. split. left. exact Hy. exact Hrho.
+    + destruct Hfree as [Hneq Hfree].
+      destruct (IHe2 x (rho_shadow rho i) Hfree) as [y [Hy Hrho]].
+      assert (y <> i) as Hyneq.
+      { intro Heq. subst.
+        unfold rho_shadow in Hrho. rewrite String.eqb_refl in Hrho. simpl in Hrho.
+        apply Hneq. exact Hrho. }
+      exists y. split.
+      * right. left. split; assumption.
+      * unfold rho_shadow in Hrho.
+        rewrite (proj2 (String.eqb_neq y i) Hyneq) in Hrho. exact Hrho.
+    + destruct Hfree as [Hneq Hfree].
+      destruct (IHe3 x (rho_shadow rho i0) Hfree) as [y [Hy Hrho]].
+      assert (y <> i0) as Hyneq.
+      { intro Heq. subst.
+        unfold rho_shadow in Hrho. rewrite String.eqb_refl in Hrho. simpl in Hrho.
+        apply Hneq. exact Hrho. }
+      exists y. split.
+      * right. right. split; assumption.
+      * unfold rho_shadow in Hrho.
+        rewrite (proj2 (String.eqb_neq y i0) Hyneq) in Hrho. exact Hrho.
+  - destruct Hfree as [Hfree | [Hfree | Hfree]].
+    + destruct (IHe1 x rho Hfree) as [y [Hy Hrho]].
+      exists y. split. left. exact Hy. exact Hrho.
+    + destruct (IHe2 x rho Hfree) as [y [Hy Hrho]].
+      exists y. split. right. left. exact Hy. exact Hrho.
+    + destruct (IHe3 x rho Hfree) as [y [Hy Hrho]].
+      exists y. split. right. right. exact Hy. exact Hrho.
+  - destruct Hfree as [Hfree | Hfree].
+    + destruct (IHe1 x rho Hfree) as [y [Hy Hrho]].
+      exists y. split. left. exact Hy. exact Hrho.
+    + destruct Hfree as [Hneq Hfree].
+      destruct (IHe2 x (rho_shadow rho i) Hfree) as [y [Hy Hrho]].
+      assert (y <> i) as Hyneq.
+      { intro Heq. subst.
+        unfold rho_shadow in Hrho. rewrite String.eqb_refl in Hrho. simpl in Hrho.
+        apply Hneq. exact Hrho. }
+      exists y. split.
+      * right. split; assumption.
+      * unfold rho_shadow in Hrho.
+        rewrite (proj2 (String.eqb_neq y i) Hyneq) in Hrho. exact Hrho.
+  - destruct (IHe x rho Hfree) as [y [Hy Hrho]].
+    exists y. split. exact Hy. exact Hrho.
+  - destruct Hfree as [Hfree | Hfree].
+    + destruct (IHe1 x rho Hfree) as [y [Hy Hrho]].
+      exists y. split. left. exact Hy. exact Hrho.
+    + destruct Hfree as [Hneq Hfree].
+      destruct (IHe2 x (rho_shadow rho i) Hfree) as [y [Hy Hrho]].
+      assert (y <> i) as Hyneq.
+      { intro Heq. subst.
+        unfold rho_shadow in Hrho. rewrite String.eqb_refl in Hrho. simpl in Hrho.
+        apply Hneq. exact Hrho. }
+      exists y. split.
+      * right. split; assumption.
+      * unfold rho_shadow in Hrho.
+        rewrite (proj2 (String.eqb_neq y i) Hyneq) in Hrho. exact Hrho.
+  - destruct (IHe x rho Hfree) as [y [Hy Hrho]].
+    exists y. split. exact Hy. exact Hrho.
+  - destruct (IHe x rho Hfree) as [y [Hy Hrho]].
+    exists y. split. exact Hy. exact Hrho.
+  - destruct Hfree as [Hfree | Hfree].
+    + destruct (IHe1 x rho Hfree) as [y [Hy Hrho]].
+      exists y. split. left. exact Hy. exact Hrho.
+    + destruct (IHe2 x rho Hfree) as [y [Hy Hrho]].
+      exists y. split. right. exact Hy. exact Hrho.
+  - destruct (IHe x rho Hfree) as [y [Hy Hrho]].
+    exists y. split. exact Hy. exact Hrho.
+  - destruct Hfree as [Hfree | Hfree].
+    + destruct (IHe1 x rho Hfree) as [y [Hy Hrho]].
+      exists y. split. left. exact Hy. exact Hrho.
+    + destruct (IHe2 x rho Hfree) as [y [Hy Hrho]].
+      exists y. split. right. exact Hy. exact Hrho.
+  - destruct (IHe x rho Hfree) as [y [Hy Hrho]].
+    exists y. split. exact Hy. exact Hrho.
+  - destruct (IHe x rho Hfree) as [y [Hy Hrho]].
+    exists y. split. exact Hy. exact Hrho.
+  - destruct (IHe x rho Hfree) as [y [Hy Hrho]].
+    exists y. split. exact Hy. exact Hrho.
+Qed.
+
+Definition env_rel (G : type_env) (rho1 rho2 : ident -> expr) : Prop :=
+  forall x T, lookup x G = Some T -> val_rel T (rho1 x) (rho2 x).
+
+Definition rho_closed_on (G : type_env) (rho : ident -> expr) : Prop :=
+  forall x T, lookup x G = Some T -> closed_expr (rho x).
+
+Definition rho_no_free_all (rho : ident -> expr) : Prop :=
+  forall x y, y <> x -> ~ free_in x (rho y).
+
+Definition rho_single (x : ident) (v : expr) : ident -> expr :=
+  fun y => if String.eqb y x then v else EVar y.
+
+Definition rho_id : ident -> expr :=
+  fun y => EVar y.
+
+Lemma rho_no_free_all_single : forall x v,
+  closed_expr v ->
+  rho_no_free_all (rho_single x v).
+Proof.
+  intros x v Hclosed.
+  unfold rho_no_free_all. intros a b Hneq.
+  unfold rho_single. destruct (String.eqb b x) eqn:Heq.
+  - apply String.eqb_eq in Heq. subst. apply (Hclosed a).
+  - simpl. intro Hfree. apply Hneq. symmetry. exact Hfree.
+Qed.
+
+Lemma env_rel_closed_left : forall G rho1 rho2,
+  env_rel G rho1 rho2 ->
+  rho_closed_on G rho1.
+Proof.
+  intros G rho1 rho2 Henv x T Hlook.
+  specialize (Henv x T Hlook) as Hrel.
+  exact (val_rel_closed_left T (rho1 x) (rho2 x) Hrel).
+Qed.
+
+Lemma env_rel_closed_right : forall G rho1 rho2,
+  env_rel G rho1 rho2 ->
+  rho_closed_on G rho2.
+Proof.
+  intros G rho1 rho2 Henv x T Hlook.
+  specialize (Henv x T Hlook) as Hrel.
+  exact (val_rel_closed_right T (rho1 x) (rho2 x) Hrel).
+Qed.
+
+Lemma closed_except_subst_rho_shadow : forall G Σ Δ rho x e T1 T2 eps,
+  has_type ((x, T1) :: G) Σ Δ e T2 eps ->
+  rho_closed_on G rho ->
+  closed_except x (subst_rho (rho_shadow rho x) e).
+Proof.
+  intros G Σ Δ rho x e T1 T2 eps Hty Hclosed y Hyneq Hfree.
+  destruct (free_in_subst_rho y (rho_shadow rho x) e Hfree) as [z [Hzfree Hzrho]].
+  destruct (free_in_context _ _ _ _ _ _ _ Hzfree Hty) as [Tz Hlook].
+  simpl in Hlook.
+  destruct (String.eqb z x) eqn:Heqzx.
+  - apply String.eqb_eq in Heqzx. subst.
+    unfold rho_shadow in Hzrho. rewrite String.eqb_refl in Hzrho. simpl in Hzrho.
+    apply Hyneq. exact Hzrho.
+  - simpl in Hlook.
+    unfold rho_shadow in Hzrho. rewrite Heqzx in Hzrho.
+    specialize (Hclosed z Tz Hlook) as Hclosedz.
+    unfold closed_expr in Hclosedz. apply (Hclosedz y) in Hzrho. contradiction.
+Qed.
+
+Lemma subst_not_free : forall x v e,
+  ~ free_in x e ->
+  [x := v] e = e.
+Proof.
+  induction e; intros Hfree; simpl in *; try reflexivity.
+  - destruct (String.eqb x i) eqn:Heq.
+    + apply String.eqb_eq in Heq. subst. exfalso. apply Hfree. reflexivity.
+    + reflexivity.
+  - destruct (String.eqb x i) eqn:Heq.
+    + reflexivity.
+    + apply String.eqb_neq in Heq.
+      f_equal. apply IHe. intro Hbody. apply Hfree. split; assumption.
+  - f_equal.
+    + apply IHe1. intro H. apply Hfree. left. exact H.
+    + apply IHe2. intro H. apply Hfree. right. exact H.
+  - f_equal.
+    + apply IHe1. intro H. apply Hfree. left. exact H.
+    + apply IHe2. intro H. apply Hfree. right. exact H.
+  - f_equal. apply IHe. intro H. apply Hfree. exact H.
+  - f_equal. apply IHe. intro H. apply Hfree. exact H.
+  - f_equal. apply IHe. intro H. apply Hfree. exact H.
+  - f_equal. apply IHe. intro H. apply Hfree. exact H.
+  - f_equal.
+    + apply IHe1. intro H. apply Hfree. left. exact H.
+    + destruct (String.eqb x i) eqn:Heq1.
+      * reflexivity.
+      * apply String.eqb_neq in Heq1.
+        apply IHe2. intro H. apply Hfree. right. left. split; assumption.
+    + destruct (String.eqb x i0) eqn:Heq2.
+      * reflexivity.
+      * apply String.eqb_neq in Heq2.
+        apply IHe3. intro H. apply Hfree. right. right. split; assumption.
+  - f_equal.
+    + apply IHe1. intro H. apply Hfree. left. exact H.
+    + apply IHe2. intro H. apply Hfree. right. left. exact H.
+    + apply IHe3. intro H. apply Hfree. right. right. exact H.
+  - f_equal.
+    + apply IHe1. intro H. apply Hfree. left. exact H.
+    + destruct (String.eqb x i) eqn:Heq.
+      * reflexivity.
+      * apply String.eqb_neq in Heq.
+        apply IHe2. intro H. apply Hfree. right. split; assumption.
+  - f_equal. apply IHe. intro H. apply Hfree. exact H.
+  - f_equal.
+    + apply IHe1. intro H. apply Hfree. left. exact H.
+    + destruct (String.eqb x i) eqn:Heq.
+      * reflexivity.
+      * apply String.eqb_neq in Heq.
+        apply IHe2. intro H. apply Hfree. right. split; assumption.
+  - f_equal. apply IHe. intro H. apply Hfree. exact H.
+  - f_equal. apply IHe. intro H. apply Hfree. exact H.
+  - f_equal.
+    + apply IHe1. intro H. apply Hfree. left. exact H.
+    + apply IHe2. intro H. apply Hfree. right. exact H.
+  - f_equal. apply IHe. intro H. apply Hfree. exact H.
+  - f_equal.
+    + apply IHe1. intro H. apply Hfree. left. exact H.
+    + apply IHe2. intro H. apply Hfree. right. exact H.
+  - f_equal. apply IHe. intro H. apply Hfree. exact H.
+  - f_equal. apply IHe. intro H. apply Hfree. exact H.
+  - f_equal. apply IHe. intro H. apply Hfree. exact H.
+Qed.
+
+Lemma rho_shadow_id : forall x,
+  rho_shadow rho_id x = rho_id.
+Proof.
+  intros x. unfold rho_shadow, rho_id.
+  apply functional_extensionality. intros y.
+  destruct (String.eqb y x); reflexivity.
+Qed.
+
+Lemma subst_rho_id : forall e,
+  subst_rho rho_id e = e.
+Proof.
+  induction e; simpl.
+  - reflexivity.
+  - reflexivity.
+  - reflexivity.
+  - reflexivity.
+  - unfold rho_id. reflexivity.
+  - rewrite rho_shadow_id. rewrite IHe. reflexivity.
+  - rewrite IHe1, IHe2. reflexivity.
+  - rewrite IHe1, IHe2. reflexivity.
+  - rewrite IHe. reflexivity.
+  - rewrite IHe. reflexivity.
+  - rewrite IHe. reflexivity.
+  - rewrite IHe. reflexivity.
+  - rewrite IHe1. rewrite rho_shadow_id. rewrite IHe2.
+    rewrite rho_shadow_id. rewrite IHe3. reflexivity.
+  - rewrite IHe1, IHe2, IHe3. reflexivity.
+  - rewrite IHe1. rewrite rho_shadow_id. rewrite IHe2. reflexivity.
+  - rewrite IHe. reflexivity.
+  - rewrite IHe1. rewrite rho_shadow_id. rewrite IHe2. reflexivity.
+  - rewrite IHe. reflexivity.
+  - rewrite IHe. reflexivity.
+  - rewrite IHe1, IHe2. reflexivity.
+  - rewrite IHe. reflexivity.
+  - rewrite IHe1, IHe2. reflexivity.
+  - rewrite IHe. reflexivity.
+  - rewrite IHe. reflexivity.
+  - rewrite IHe. reflexivity.
+Qed.
+
+Lemma rho_shadow_single_eq : forall x v i,
+  x <> i ->
+  rho_shadow (rho_single x v) i = rho_single x v.
+Proof.
+  intros x v i Hneq.
+  unfold rho_shadow, rho_single.
+  apply functional_extensionality. intros y.
+  destruct (String.eqb y i) eqn:Heqyi.
+  - apply String.eqb_eq in Heqyi. subst.
+    assert (String.eqb i x = false) as Heqix.
+    { apply (proj2 (String.eqb_neq i x)).
+      intro Heq. apply Hneq. symmetry. exact Heq. }
+    rewrite Heqix. reflexivity.
+  - reflexivity.
+Qed.
+
+Lemma rho_shadow_single_id : forall x v,
+  rho_shadow (rho_single x v) x = rho_id.
+Proof.
+  intros x v.
+  unfold rho_shadow, rho_single, rho_id.
+  apply functional_extensionality. intros y.
+  destruct (String.eqb y x) eqn:Heqyx; reflexivity.
+Qed.
+
+Lemma subst_rho_single : forall e x v,
+  subst_rho (rho_single x v) e = [x := v] e.
+Proof.
+  induction e; intros x v; simpl; try reflexivity.
+  - unfold rho_single. destruct (String.eqb x i) eqn:Heqxi; simpl.
+    + apply String.eqb_eq in Heqxi. subst. rewrite String.eqb_refl. reflexivity.
+    + apply String.eqb_neq in Heqxi.
+      assert (String.eqb i x = false) as Heqix.
+      { destruct (String.eqb i x) eqn:Heqix; auto.
+        apply String.eqb_eq in Heqix. subst.
+        exfalso. apply Heqxi. reflexivity. }
+      rewrite Heqix. reflexivity.
+  - destruct (String.eqb x i) eqn:Heq.
+    + apply String.eqb_eq in Heq. subst.
+      rewrite rho_shadow_single_id. rewrite subst_rho_id. reflexivity.
+    + apply (proj1 (String.eqb_neq x i)) in Heq.
+      rewrite rho_shadow_single_eq by assumption. rewrite IHe. reflexivity.
+  - rewrite IHe1, IHe2. reflexivity.
+  - rewrite IHe1, IHe2. reflexivity.
+  - rewrite IHe. reflexivity.
+  - rewrite IHe. reflexivity.
+  - rewrite IHe. reflexivity.
+  - rewrite IHe. reflexivity.
+  - rewrite IHe1.
+    destruct (String.eqb x i) eqn:Heq1.
+    + apply String.eqb_eq in Heq1. subst.
+      rewrite rho_shadow_single_id. rewrite subst_rho_id.
+      destruct (String.eqb i i0) eqn:Heq2.
+      * apply String.eqb_eq in Heq2. subst.
+        rewrite rho_shadow_single_id. rewrite subst_rho_id. reflexivity.
+      * apply (proj1 (String.eqb_neq i i0)) in Heq2.
+        rewrite rho_shadow_single_eq by assumption. rewrite IHe3. reflexivity.
+    + apply (proj1 (String.eqb_neq x i)) in Heq1.
+      rewrite rho_shadow_single_eq by assumption. rewrite IHe2.
+      destruct (String.eqb x i0) eqn:Heq2.
+      * apply String.eqb_eq in Heq2. subst.
+        rewrite rho_shadow_single_id. rewrite subst_rho_id. reflexivity.
+      * apply (proj1 (String.eqb_neq x i0)) in Heq2.
+        rewrite rho_shadow_single_eq by assumption. rewrite IHe3. reflexivity.
+  - rewrite IHe1, IHe2, IHe3. reflexivity.
+  - rewrite IHe1.
+    destruct (String.eqb x i) eqn:Heq.
+    + apply String.eqb_eq in Heq. subst.
+      rewrite rho_shadow_single_id. rewrite subst_rho_id. reflexivity.
+    + apply (proj1 (String.eqb_neq x i)) in Heq.
+      rewrite rho_shadow_single_eq by assumption. rewrite IHe2. reflexivity.
+  - rewrite IHe. reflexivity.
+  - rewrite IHe1.
+    destruct (String.eqb x i) eqn:Heq.
+    + apply String.eqb_eq in Heq. subst.
+      rewrite rho_shadow_single_id. rewrite subst_rho_id. reflexivity.
+    + apply (proj1 (String.eqb_neq x i)) in Heq.
+      rewrite rho_shadow_single_eq by assumption. rewrite IHe2. reflexivity.
+  - rewrite IHe. reflexivity.
+  - rewrite IHe. reflexivity.
+  - rewrite IHe1, IHe2. reflexivity.
+  - rewrite IHe. reflexivity.
+  - rewrite IHe1, IHe2. reflexivity.
+  - rewrite IHe. reflexivity.
+  - rewrite IHe. reflexivity.
+  - rewrite IHe. reflexivity.
+Qed.
+
+Lemma rho_shadow_extend_same : forall rho x v,
+  rho_shadow (rho_extend rho x v) x = rho_shadow rho x.
+Proof.
+  intros rho x v. unfold rho_shadow, rho_extend.
+  apply functional_extensionality. intros y.
+  destruct (String.eqb y x) eqn:Heq; reflexivity.
+Qed.
+
+Lemma rho_shadow_shadow_same : forall rho x,
+  rho_shadow (rho_shadow rho x) x = rho_shadow rho x.
+Proof.
+  intros rho x. unfold rho_shadow.
+  apply functional_extensionality. intros y.
+  destruct (String.eqb y x) eqn:Heq; reflexivity.
+Qed.
+
+Lemma rho_shadow_shadow_comm : forall rho x y,
+  x <> y ->
+  rho_shadow (rho_shadow rho x) y = rho_shadow (rho_shadow rho y) x.
+Proof.
+  intros rho x y Hneq. unfold rho_shadow.
+  apply functional_extensionality. intros z.
+  destruct (String.eqb z y) eqn:Heqzy;
+  destruct (String.eqb z x) eqn:Heqzx; try reflexivity.
+  all: apply String.eqb_eq in Heqzy; apply String.eqb_eq in Heqzx; subst;
+    exfalso; apply Hneq; reflexivity.
+Qed.
+
+Lemma rho_shadow_extend_comm : forall rho x y v,
+  x <> y ->
+  rho_shadow (rho_extend rho x v) y = rho_extend (rho_shadow rho y) x v.
+Proof.
+  intros rho x y v Hneq. unfold rho_shadow, rho_extend.
+  apply functional_extensionality. intros z.
+  destruct (String.eqb z y) eqn:Heqzy;
+  destruct (String.eqb z x) eqn:Heqzx; try reflexivity.
+  all: apply String.eqb_eq in Heqzy; apply String.eqb_eq in Heqzx; subst;
+    exfalso; apply Hneq; reflexivity.
+Qed.
+
+Lemma rho_no_free_extend : forall rho x v,
+  rho_no_free_all rho ->
+  closed_expr v ->
+  rho_no_free_all (rho_extend rho x v).
+Proof.
+  intros rho x v Hno Hclosed.
+  unfold rho_no_free_all in *. intros a b Hneq.
+  unfold rho_extend. destruct (String.eqb b x) eqn:Heq.
+  - apply String.eqb_eq in Heq. subst. apply Hclosed.
+  - apply Hno. exact Hneq.
+Qed.
+
+Lemma rho_no_free_shadow : forall rho x,
+  rho_no_free_all rho ->
+  rho_no_free_all (rho_shadow rho x).
+Proof.
+  intros rho x Hno.
+  unfold rho_no_free_all in *. intros a b Hneq.
+  unfold rho_shadow. destruct (String.eqb b x) eqn:Heq.
+  - simpl. intro Hfree. apply Hneq. symmetry. exact Hfree.
+  - apply Hno. exact Hneq.
+Qed.
+
+Lemma subst_rho_extend : forall rho x v e,
+  rho_no_free_all rho ->
+  [x := v] (subst_rho (rho_shadow rho x) e) =
+  subst_rho (rho_extend rho x v) e.
+Proof.
+  intros rho0 x0 v0 e Hno.
+  revert rho0 x0 v0 Hno.
+  induction e; intros rho0 x0 v0 Hno; simpl; try reflexivity.
+  - destruct (String.eqb i x0) eqn:Heq; simpl.
+    + apply String.eqb_eq in Heq. subst.
+      unfold rho_shadow, rho_extend. simpl.
+      rewrite String.eqb_refl. simpl. rewrite String.eqb_refl. reflexivity.
+    + assert (i <> x0) as Hneq by (apply String.eqb_neq; exact Heq).
+      unfold rho_shadow, rho_extend.
+      rewrite Heq.
+      simpl.
+      apply subst_not_free.
+      apply (Hno x0 i). exact Hneq.
+  - destruct (String.eqb x0 i) eqn:Heq.
+    + apply String.eqb_eq in Heq. subst.
+      simpl. rewrite rho_shadow_shadow_same. rewrite rho_shadow_extend_same. reflexivity.
+    + apply String.eqb_neq in Heq.
+      simpl.
+      rewrite (rho_shadow_shadow_comm rho0 x0 i) by assumption.
+      rewrite (rho_shadow_extend_comm rho0 x0 i v0) by assumption.
+      rewrite (IHe (rho_shadow rho0 i) x0 v0 (rho_no_free_shadow rho0 i Hno)).
+      reflexivity.
+  - rewrite (IHe1 rho0 x0 v0 Hno), (IHe2 rho0 x0 v0 Hno). reflexivity.
+  - rewrite (IHe1 rho0 x0 v0 Hno), (IHe2 rho0 x0 v0 Hno). reflexivity.
+  - rewrite (IHe rho0 x0 v0 Hno). reflexivity.
+  - rewrite (IHe rho0 x0 v0 Hno). reflexivity.
+  - rewrite (IHe rho0 x0 v0 Hno). reflexivity.
+  - rewrite (IHe rho0 x0 v0 Hno). reflexivity.
+  - rewrite (IHe1 rho0 x0 v0 Hno).
+    destruct (String.eqb x0 i) eqn:Heq1.
+    + apply String.eqb_eq in Heq1. subst.
+      simpl.
+      rewrite rho_shadow_shadow_same. rewrite rho_shadow_extend_same.
+      destruct (String.eqb i i0) eqn:Heq2.
+      * apply String.eqb_eq in Heq2. subst.
+        simpl.
+        rewrite rho_shadow_shadow_same. rewrite rho_shadow_extend_same. reflexivity.
+      * assert (i <> i0) as Hneq2 by (apply String.eqb_neq; exact Heq2).
+        simpl.
+        rewrite (rho_shadow_shadow_comm rho0 i i0) by assumption.
+        rewrite (rho_shadow_extend_comm rho0 i i0 v0) by assumption.
+        rewrite (IHe3 (rho_shadow rho0 i0) i v0 (rho_no_free_shadow rho0 i0 Hno)).
+        reflexivity.
+    + assert (x0 <> i) as Hneq1 by (apply String.eqb_neq; exact Heq1).
+      simpl.
+      rewrite (rho_shadow_shadow_comm rho0 x0 i) by assumption.
+      rewrite (rho_shadow_extend_comm rho0 x0 i v0) by assumption.
+      rewrite (IHe2 (rho_shadow rho0 i) x0 v0 (rho_no_free_shadow rho0 i Hno)).
+      destruct (String.eqb x0 i0) eqn:Heq2.
+      * apply String.eqb_eq in Heq2. subst.
+        simpl.
+        rewrite rho_shadow_shadow_same. rewrite rho_shadow_extend_same. reflexivity.
+      * assert (x0 <> i0) as Hneq2 by (apply String.eqb_neq; exact Heq2).
+        simpl.
+        rewrite (rho_shadow_shadow_comm rho0 x0 i0) by assumption.
+        rewrite (rho_shadow_extend_comm rho0 x0 i0 v0) by assumption.
+        rewrite (IHe3 (rho_shadow rho0 i0) x0 v0 (rho_no_free_shadow rho0 i0 Hno)).
+        reflexivity.
+  - rewrite (IHe1 rho0 x0 v0 Hno). rewrite (IHe2 rho0 x0 v0 Hno). rewrite (IHe3 rho0 x0 v0 Hno). reflexivity.
+  - destruct (String.eqb x0 i) eqn:Heq.
+    + apply String.eqb_eq in Heq. subst.
+      simpl.
+      rewrite (IHe1 rho0 i v0 Hno).
+      rewrite rho_shadow_shadow_same. rewrite rho_shadow_extend_same. reflexivity.
+    + apply String.eqb_neq in Heq.
+      simpl.
+      rewrite (IHe1 rho0 x0 v0 Hno).
+      rewrite (rho_shadow_shadow_comm rho0 x0 i) by assumption.
+      rewrite (rho_shadow_extend_comm rho0 x0 i v0) by assumption.
+      rewrite (IHe2 (rho_shadow rho0 i) x0 v0 (rho_no_free_shadow rho0 i Hno)).
+      reflexivity.
+  - rewrite (IHe rho0 x0 v0 Hno). reflexivity.
+  - destruct (String.eqb x0 i) eqn:Heq.
+    + apply String.eqb_eq in Heq. subst.
+      simpl.
+      rewrite (IHe1 rho0 i v0 Hno).
+      rewrite rho_shadow_shadow_same. rewrite rho_shadow_extend_same. reflexivity.
+    + apply String.eqb_neq in Heq.
+      simpl.
+      rewrite (IHe1 rho0 x0 v0 Hno).
+      rewrite (rho_shadow_shadow_comm rho0 x0 i) by assumption.
+      rewrite (rho_shadow_extend_comm rho0 x0 i v0) by assumption.
+      rewrite (IHe2 (rho_shadow rho0 i) x0 v0 (rho_no_free_shadow rho0 i Hno)).
+      reflexivity.
+  - rewrite (IHe rho0 x0 v0 Hno). reflexivity.
+  - rewrite (IHe rho0 x0 v0 Hno). reflexivity.
+  - rewrite (IHe1 rho0 x0 v0 Hno). rewrite (IHe2 rho0 x0 v0 Hno). reflexivity.
+  - rewrite (IHe rho0 x0 v0 Hno). reflexivity.
+  - rewrite (IHe1 rho0 x0 v0 Hno). rewrite (IHe2 rho0 x0 v0 Hno). reflexivity.
+  - rewrite (IHe rho0 x0 v0 Hno). reflexivity.
+  - rewrite (IHe rho0 x0 v0 Hno). reflexivity.
+  - rewrite (IHe rho0 x0 v0 Hno). reflexivity.
+Qed.
+
+Lemma env_rel_extend : forall G rho1 rho2 x T v1 v2,
+  env_rel G rho1 rho2 ->
+  val_rel T v1 v2 ->
+  env_rel ((x, T) :: G) (rho_extend rho1 x v1) (rho_extend rho2 x v2).
+Proof.
+  intros G rho1 rho2 x T v1 v2 Henv Hv.
+  unfold env_rel in *. intros y Ty Hlook.
+  simpl in Hlook.
+  destruct (String.eqb y x) eqn:Heq.
+  - apply String.eqb_eq in Heq. subst.
+    inversion Hlook; subst.
+    unfold rho_extend.
+    destruct (String.eqb x x) eqn:Heqxx.
+    * simpl. exact Hv.
+    * apply String.eqb_neq in Heqxx. exfalso. apply Heqxx. reflexivity.
+  - unfold rho_extend. rewrite Heq. apply Henv. assumption.
+Qed.
+
+(** ** Multi-step Lemmas *)
+
+Lemma multi_step_trans : forall cfg1 cfg2 cfg3,
+  cfg1 -->* cfg2 ->
+  cfg2 -->* cfg3 ->
+  cfg1 -->* cfg3.
+Proof.
+  intros cfg1 cfg2 cfg3 H12 H23.
+  induction H12.
+  - assumption.
+  - eapply MS_Step; eauto.
+Qed.
+
+Lemma multi_step_app1 : forall e1 e1' e2 st st' ctx ctx',
+  (e1, st, ctx) -->* (e1', st', ctx') ->
+  (EApp e1 e2, st, ctx) -->* (EApp e1' e2, st', ctx').
+Proof.
+  intros e1 e1' e2 st st' ctx ctx' H.
+  dependent induction H.
+  - apply MS_Refl.
+  - destruct cfg2 as [[e_mid st_mid] ctx_mid].
+    eapply MS_Step.
+    + apply ST_App1. exact H.
+    + apply (IHmulti_step e_mid e1' st_mid st' ctx_mid ctx'); reflexivity.
+Qed.
+
+Lemma multi_step_app2 : forall v1 e2 e2' st st' ctx ctx',
+  value v1 ->
+  (e2, st, ctx) -->* (e2', st', ctx') ->
+  (EApp v1 e2, st, ctx) -->* (EApp v1 e2', st', ctx').
+Proof.
+  intros v1 e2 e2' st st' ctx ctx' Hv H.
+  dependent induction H.
+  - apply MS_Refl.
+  - destruct cfg2 as [[e_mid st_mid] ctx_mid].
+    eapply MS_Step.
+    + apply ST_App2; eauto.
+    + apply (IHmulti_step e_mid e2' st_mid st' ctx_mid ctx').
+      * exact Hv.
+      * exact eq_refl.
+      * exact eq_refl.
+Qed.
+
+Lemma multi_step_pair1 : forall e1 e1' e2 st st' ctx ctx',
+  (e1, st, ctx) -->* (e1', st', ctx') ->
+  (EPair e1 e2, st, ctx) -->* (EPair e1' e2, st', ctx').
+Proof.
+  intros e1 e1' e2 st st' ctx ctx' H.
+  dependent induction H.
+  - apply MS_Refl.
+  - destruct cfg2 as [[e_mid st_mid] ctx_mid].
+    eapply MS_Step.
+    + apply ST_Pair1. exact H.
+    + apply (IHmulti_step e_mid e1' st_mid st' ctx_mid ctx'); reflexivity.
+Qed.
+
+Lemma multi_step_pair2 : forall v1 e2 e2' st st' ctx ctx',
+  value v1 ->
+  (e2, st, ctx) -->* (e2', st', ctx') ->
+  (EPair v1 e2, st, ctx) -->* (EPair v1 e2', st', ctx').
+Proof.
+  intros v1 e2 e2' st st' ctx ctx' Hv H.
+  dependent induction H.
+  - apply MS_Refl.
+  - destruct cfg2 as [[e_mid st_mid] ctx_mid].
+    eapply MS_Step.
+    + apply ST_Pair2; eauto.
+    + apply (IHmulti_step e_mid e2' st_mid st' ctx_mid ctx').
+      * exact Hv.
+      * exact eq_refl.
+      * exact eq_refl.
+Qed.
+
+Lemma multi_step_fst : forall e e' st st' ctx ctx',
+  (e, st, ctx) -->* (e', st', ctx') ->
+  (EFst e, st, ctx) -->* (EFst e', st', ctx').
+Proof.
+  intros e e' st st' ctx ctx' H.
+  dependent induction H.
+  - apply MS_Refl.
+  - destruct cfg2 as [[e_mid st_mid] ctx_mid].
+    eapply MS_Step.
+    + apply ST_FstStep. exact H.
+    + apply (IHmulti_step e_mid e' st_mid st' ctx_mid ctx'); reflexivity.
+Qed.
+
+Lemma multi_step_snd : forall e e' st st' ctx ctx',
+  (e, st, ctx) -->* (e', st', ctx') ->
+  (ESnd e, st, ctx) -->* (ESnd e', st', ctx').
+Proof.
+  intros e e' st st' ctx ctx' H.
+  dependent induction H.
+  - apply MS_Refl.
+  - destruct cfg2 as [[e_mid st_mid] ctx_mid].
+    eapply MS_Step.
+    + apply ST_SndStep. exact H.
+    + apply (IHmulti_step e_mid e' st_mid st' ctx_mid ctx'); reflexivity.
+Qed.
+
+Lemma multi_step_inl : forall e e' T st st' ctx ctx',
+  (e, st, ctx) -->* (e', st', ctx') ->
+  (EInl e T, st, ctx) -->* (EInl e' T, st', ctx').
+Proof.
+  intros e e' T st st' ctx ctx' H.
+  dependent induction H.
+  - apply MS_Refl.
+  - destruct cfg2 as [[e_mid st_mid] ctx_mid].
+    eapply MS_Step.
+    + apply ST_InlStep. exact H.
+    + apply (IHmulti_step e_mid e' st_mid st' ctx_mid ctx'); reflexivity.
+Qed.
+
+Lemma multi_step_inr : forall e e' T st st' ctx ctx',
+  (e, st, ctx) -->* (e', st', ctx') ->
+  (EInr e T, st, ctx) -->* (EInr e' T, st', ctx').
+Proof.
+  intros e e' T st st' ctx ctx' H.
+  dependent induction H.
+  - apply MS_Refl.
+  - destruct cfg2 as [[e_mid st_mid] ctx_mid].
+    eapply MS_Step.
+    + apply ST_InrStep. exact H.
+    + apply (IHmulti_step e_mid e' st_mid st' ctx_mid ctx'); reflexivity.
+Qed.
+
+Lemma multi_step_case : forall e e' x1 e1 x2 e2 st st' ctx ctx',
+  (e, st, ctx) -->* (e', st', ctx') ->
+  (ECase e x1 e1 x2 e2, st, ctx) -->* (ECase e' x1 e1 x2 e2, st', ctx').
+Proof.
+  intros e e' x1 e1 x2 e2 st st' ctx ctx' H.
+  dependent induction H.
+  - apply MS_Refl.
+  - destruct cfg2 as [[e_mid st_mid] ctx_mid].
+    eapply MS_Step.
+    + apply ST_CaseStep. exact H.
+    + apply (IHmulti_step e_mid e' st_mid st' ctx_mid ctx'); reflexivity.
+Qed.
+
+Lemma multi_step_if : forall e1 e1' e2 e3 st st' ctx ctx',
+  (e1, st, ctx) -->* (e1', st', ctx') ->
+  (EIf e1 e2 e3, st, ctx) -->* (EIf e1' e2 e3, st', ctx').
+Proof.
+  intros e1 e1' e2 e3 st st' ctx ctx' H.
+  dependent induction H.
+  - apply MS_Refl.
+  - destruct cfg2 as [[e_mid st_mid] ctx_mid].
+    eapply MS_Step.
+    + apply ST_IfStep. exact H.
+    + apply (IHmulti_step e_mid e1' st_mid st' ctx_mid ctx'); reflexivity.
+Qed.
+
+Lemma multi_step_let : forall x e1 e1' e2 st st' ctx ctx',
+  (e1, st, ctx) -->* (e1', st', ctx') ->
+  (ELet x e1 e2, st, ctx) -->* (ELet x e1' e2, st', ctx').
+Proof.
+  intros x e1 e1' e2 st st' ctx ctx' H.
+  dependent induction H.
+  - apply MS_Refl.
+  - destruct cfg2 as [[e_mid st_mid] ctx_mid].
+    eapply MS_Step.
+    + apply ST_LetStep. exact H.
+    + apply (IHmulti_step e_mid e1' st_mid st' ctx_mid ctx'); reflexivity.
+Qed.
+
+Lemma exp_rel_of_val_rel : forall T v1 v2,
+  val_rel T v1 v2 ->
+  exp_rel T v1 v2.
+Proof.
+  intros T v1 v2 Hrel st1 st2 ctx.
+  exists v1, v2, st1, st2, ctx.
+  split.
+  - apply MS_Refl.
+  - split.
+    + apply MS_Refl.
+    + exact Hrel.
+Qed.
 
 Fixpoint lookup_val (x : ident) (s : list (ident * expr)) : option expr :=
   match s with
@@ -88,21 +936,418 @@ Definition subst_rel (G : type_env) (s1 s2 : list (ident * expr)) : Prop :=
       lookup_val x s2 = Some v2 /\ 
       val_rel T v1 v2.
 
+(** ** Fundamental Theorem *)
+
+Theorem logical_relation : forall G e T eps rho1 rho2,
+  has_type G nil Public e T eps ->
+  env_rel G rho1 rho2 ->
+  rho_no_free_all rho1 ->
+  rho_no_free_all rho2 ->
+  exp_rel T (subst_rho rho1 e) (subst_rho rho2 e).
+Proof.
+  intros G e T eps rho1 rho2 Hty.
+  generalize dependent rho1.
+  generalize dependent rho2.
+  induction Hty; intros rho2 rho1 Henv Hno2 Hno1; simpl.
+  - (* T_Unit *)
+    apply exp_rel_of_val_rel. simpl.
+    repeat split; try constructor; try reflexivity; intros x; simpl; auto.
+  - (* T_Bool *)
+    apply exp_rel_of_val_rel. simpl.
+    repeat split.
+    + constructor.
+    + constructor.
+    + intros x; simpl; auto.
+    + intros x; simpl; auto.
+    + exists b. auto.
+  - (* T_Int *)
+    apply exp_rel_of_val_rel. simpl.
+    repeat split.
+    + constructor.
+    + constructor.
+    + intros x; simpl; auto.
+    + intros x; simpl; auto.
+    + exists n. auto.
+  - (* T_String *)
+    apply exp_rel_of_val_rel. simpl.
+    repeat split.
+    + constructor.
+    + constructor.
+    + intros x; simpl; auto.
+    + intros x; simpl; auto.
+    + exists s. auto.
+  - apply exp_rel_of_val_rel. apply Henv. assumption.
+  - (* T_Lam *)
+    apply exp_rel_of_val_rel.
+    simpl.
+    repeat split.
+    + apply VLam.
+    + apply VLam.
+    + apply closed_expr_lam. eapply closed_except_subst_rho_shadow.
+      { match goal with H : has_type _ _ _ _ _ _ |- _ => exact H end. }
+      { apply (env_rel_closed_left _ _ _ Henv). }
+    + apply closed_expr_lam. eapply closed_except_subst_rho_shadow.
+      { match goal with H : has_type _ _ _ _ _ _ |- _ => exact H end. }
+      { apply (env_rel_closed_right _ _ _ Henv). }
+    + intros vx vy Hrelxy st1 st2 ctx.
+      pose proof (env_rel_extend _ _ _ x T1 vx vy Henv Hrelxy) as Henv'.
+      assert (rho_no_free_all (rho_extend rho1 x vx)) as Hno1'.
+      { apply rho_no_free_extend. assumption. apply (val_rel_closed_left _ _ _ Hrelxy). }
+      assert (rho_no_free_all (rho_extend rho2 x vy)) as Hno2'.
+      { apply rho_no_free_extend. assumption. apply (val_rel_closed_right _ _ _ Hrelxy). }
+      specialize (IHHty _ _ Henv' Hno1' Hno2').
+      unfold exp_rel in IHHty.
+      specialize (IHHty st1 st2 ctx).
+      destruct IHHty as [v1' [v2' [st1' [st2' [ctx' [Hms1 [Hms2 Hval]]]]]]].
+      
+      rewrite <- (subst_rho_extend rho1 x vx e Hno2) in Hms1.
+      rewrite <- (subst_rho_extend rho2 x vy e Hno1) in Hms2.
+      
+      exists v1', v2', st1', st2', ctx'.
+      split.
+      * eapply MS_Step.
+        -- apply ST_AppAbs. apply (val_rel_value_left _ _ _ Hrelxy).
+        -- exact Hms1.
+      * split.
+        -- eapply MS_Step.
+           ++ apply ST_AppAbs. apply (val_rel_value_right _ _ _ Hrelxy).
+           ++ exact Hms2.
+        -- exact Hval.
+  - (* T_App *)
+    unfold exp_rel in IHHty1.
+    specialize (IHHty1 rho2 rho1 Henv Hno2 Hno1).
+    unfold exp_rel in IHHty2.
+    specialize (IHHty2 rho2 rho1 Henv Hno2 Hno1).
+    intros st1 st2 ctx.
+    destruct (IHHty1 st1 st2 ctx) as
+      [vf1 [vf2 [st1' [st2' [ctx' [Hmsf1 [Hmsf2 Hrelf]]]]]]].
+    destruct (IHHty2 st1' st2' ctx') as
+      [va1 [va2 [st1'' [st2'' [ctx'' [Hmsa1 [Hmsa2 Hrela]]]]]]].
+    simpl in Hrelf.
+    destruct Hrelf as [Hf1 Hrelf1].
+    destruct Hrelf1 as [Hf2 Hrelf2].
+    destruct Hrelf2 as [_ Hrelf3].
+    destruct Hrelf3 as [_ Hfrel].
+    destruct (Hfrel va1 va2 Hrela st1'' st2'' ctx'') as
+      [vr1 [vr2 [st1''' [st2''' [ctx''' [Hms1 [Hms2 Hrelr]]]]]]].
+    exists vr1, vr2, st1''', st2''', ctx'''.
+    split.
+    + eapply multi_step_trans with (cfg2 := (EApp vf1 (subst_rho rho1 e2), st1', ctx')).
+      { apply multi_step_app1. exact Hmsf1. }
+      { eapply multi_step_trans with (cfg2 := (EApp vf1 va1, st1'', ctx'')).
+        { apply multi_step_app2; assumption. }
+        { exact Hms1. }
+      }
+    + split.
+      { eapply multi_step_trans with (cfg2 := (EApp vf2 (subst_rho rho2 e2), st2', ctx')).
+        { apply multi_step_app1. exact Hmsf2. }
+        { eapply multi_step_trans with (cfg2 := (EApp vf2 va2, st2'', ctx'')).
+           { apply multi_step_app2; assumption. }
+           { exact Hms2. }
+        }
+      }
+      { exact Hrelr. }
+  - (* T_Pair *)
+    unfold exp_rel in IHHty1. specialize (IHHty1 rho2 rho1 Henv Hno2 Hno1).
+    unfold exp_rel in IHHty2. specialize (IHHty2 rho2 rho1 Henv Hno2 Hno1).
+    intros st1 st2 ctx.
+    destruct (IHHty1 st1 st2 ctx) as
+      [v1a [v2a [st1' [st2' [ctx' [Hms1a [Hms2a Hrela]]]]]]].
+    destruct (IHHty2 st1' st2' ctx') as
+      [v1b [v2b [st1'' [st2'' [ctx'' [Hms1b [Hms2b Hrelb]]]]]]].
+    exists (EPair v1a v1b), (EPair v2a v2b), st1'', st2'', ctx''.
+    split.
+    + eapply multi_step_trans.
+      * apply multi_step_pair1. exact Hms1a.
+      * eapply multi_step_pair2.
+        { apply (val_rel_value_left _ _ _ Hrela). }
+        { exact Hms1b. }
+    + split.
+      * eapply multi_step_trans.
+        -- apply multi_step_pair1. exact Hms2a.
+        -- eapply multi_step_pair2.
+           { apply (val_rel_value_right _ _ _ Hrela). }
+           { exact Hms2b. }
+      * unfold val_rel. repeat split.
+        -- apply VPair. apply (val_rel_value_left _ _ _ Hrela). apply (val_rel_value_left _ _ _ Hrelb).
+        -- apply VPair. apply (val_rel_value_right _ _ _ Hrela). apply (val_rel_value_right _ _ _ Hrelb).
+        -- apply closed_expr_pair. apply (val_rel_closed_left _ _ _ Hrela). apply (val_rel_closed_left _ _ _ Hrelb).
+        -- apply closed_expr_pair. apply (val_rel_closed_right _ _ _ Hrela). apply (val_rel_closed_right _ _ _ Hrelb).
+        -- exists v1a, v1b, v2a, v2b.
+           repeat split; try reflexivity; assumption.
+  - (* T_Fst *)
+    unfold exp_rel in IHHty. specialize (IHHty rho2 rho1 Henv Hno2 Hno1).
+    intros st1 st2 ctx.
+    destruct (IHHty st1 st2 ctx) as
+      [vp1 [vp2 [st1' [st2' [ctx' [Hms1 [Hms2 Hrelp]]]]]]].
+    destruct Hrelp as [Hp1 [Hp2 [Hc1 [Hc2 Hrelp']]]].
+    destruct Hrelp' as [a1 [b1 [a2 [b2 [Heq1 [Heq2 [Hrela Hrelb]]]]]]].
+    subst.
+    exists a1, a2, st1', st2', ctx'.
+    split.
+    + eapply multi_step_trans.
+      * apply multi_step_fst. exact Hms1.
+      * eapply MS_Step.
+        -- apply ST_Fst.
+           ++ apply (val_rel_value_left _ _ _ Hrela).
+           ++ apply (val_rel_value_left _ _ _ Hrelb).
+        -- apply MS_Refl.
+    + split.
+      * eapply multi_step_trans.
+        -- apply multi_step_fst. exact Hms2.
+        -- eapply MS_Step.
+           ++ apply ST_Fst.
+              ** apply (val_rel_value_right _ _ _ Hrela).
+              ** apply (val_rel_value_right _ _ _ Hrelb).
+           ++ apply MS_Refl.
+      * exact Hrela.
+  - (* T_Snd *)
+    unfold exp_rel in IHHty. specialize (IHHty rho2 rho1 Henv Hno2 Hno1).
+    intros st1 st2 ctx.
+    destruct (IHHty st1 st2 ctx) as
+      [vp1 [vp2 [st1' [st2' [ctx' [Hms1 [Hms2 Hrelp]]]]]]].
+    destruct Hrelp as [Hp1 [Hp2 [Hc1 [Hc2 Hrelp']]]].
+    destruct Hrelp' as [a1 [b1 [a2 [b2 [Heq1 [Heq2 [Hrela Hrelb]]]]]]].
+    subst.
+    exists b1, b2, st1', st2', ctx'.
+    split.
+    + eapply multi_step_trans.
+      * apply multi_step_snd. exact Hms1.
+      * eapply MS_Step.
+        -- apply ST_Snd.
+           ++ apply (val_rel_value_left _ _ _ Hrela).
+           ++ apply (val_rel_value_left _ _ _ Hrelb).
+        -- apply MS_Refl.
+    + split.
+      * eapply multi_step_trans.
+        -- apply multi_step_snd. exact Hms2.
+        -- eapply MS_Step.
+           ++ apply ST_Snd.
+              ** apply (val_rel_value_right _ _ _ Hrela).
+              ** apply (val_rel_value_right _ _ _ Hrelb).
+           ++ apply MS_Refl.
+      * exact Hrelb.
+  - (* T_Inl *)
+    unfold exp_rel in IHHty. specialize (IHHty rho2 rho1 Henv Hno2 Hno1).
+    intros st1 st2 ctx.
+    destruct (IHHty st1 st2 ctx) as
+      [v1 [v2 [st1' [st2' [ctx' [Hms1 [Hms2 Hrelv]]]]]]].
+    exists (EInl v1 T2), (EInl v2 T2), st1', st2', ctx'.
+    split.
+    + eapply multi_step_trans.
+      * apply multi_step_inl. exact Hms1.
+      * apply MS_Refl.
+    + split.
+      * eapply multi_step_trans.
+        -- apply multi_step_inl. exact Hms2.
+        -- apply MS_Refl.
+      * unfold val_rel. repeat split.
+        -- apply VInl. apply (val_rel_value_left _ _ _ Hrelv).
+        -- apply VInl. apply (val_rel_value_right _ _ _ Hrelv).
+        -- apply closed_expr_inl. apply (val_rel_closed_left _ _ _ Hrelv).
+        -- apply closed_expr_inl. apply (val_rel_closed_right _ _ _ Hrelv).
+        -- left. exists v1, v2. repeat split; try reflexivity; exact Hrelv.
+  - (* T_Inr *)
+    unfold exp_rel in IHHty. specialize (IHHty rho2 rho1 Henv Hno2 Hno1).
+    intros st1 st2 ctx.
+    destruct (IHHty st1 st2 ctx) as
+      [v1 [v2 [st1' [st2' [ctx' [Hms1 [Hms2 Hrelv]]]]]]].
+    exists (EInr v1 T1), (EInr v2 T1), st1', st2', ctx'.
+    split.
+    + eapply multi_step_trans.
+      * apply multi_step_inr. exact Hms1.
+      * apply MS_Refl.
+    + split.
+      * eapply multi_step_trans.
+        -- apply multi_step_inr. exact Hms2.
+        -- apply MS_Refl.
+      * unfold val_rel. repeat split.
+        -- apply VInr. apply (val_rel_value_left _ _ _ Hrelv).
+        -- apply VInr. apply (val_rel_value_right _ _ _ Hrelv).
+        -- apply closed_expr_inr. apply (val_rel_closed_left _ _ _ Hrelv).
+        -- apply closed_expr_inr. apply (val_rel_closed_right _ _ _ Hrelv).
+        -- right. exists v1, v2. repeat split; try reflexivity; exact Hrelv.
+  - (* T_Case *)
+    unfold exp_rel in IHHty1. specialize (IHHty1 rho2 rho1 Henv Hno2 Hno1).
+    intros st1 st2 ctx.
+    destruct (IHHty1 st1 st2 ctx) as
+      [v1 [v2 [st1' [st2' [ctx' [Hms1 [Hms2 Hrelv]]]]]]].
+    destruct Hrelv as [Hv1 [Hv2 [Hc1 [Hc2 Hsum]]]].
+    destruct Hsum as [[a1 [a2 [Heq1 [Heq2 Hrela]]]] | [b1 [b2 [Heq1 [Heq2 Hrelb]]]]];
+      subst.
+    + (* inl *)
+      pose proof (val_rel_value_left _ _ _ Hrela) as Ha1.
+      pose proof (val_rel_value_right _ _ _ Hrela) as Ha2.
+      pose proof (env_rel_extend _ _ _ x1 T1 a1 a2 Henv Hrela) as Henv'.
+      assert (rho_no_free_all (rho_extend rho1 x1 a1)) as Hno1'.
+      { apply rho_no_free_extend; assumption. }
+      assert (rho_no_free_all (rho_extend rho2 x1 a2)) as Hno2'.
+      { apply rho_no_free_extend; assumption. }
+      specialize (IHHty2 _ _ Henv' Hno1' Hno2') as Hexp.
+      unfold exp_rel in Hexp.
+      specialize (Hexp st1' st2' ctx').
+      destruct Hexp as [vr1 [vr2 [st1'' [st2'' [ctx'' [Hms1' [Hms2' Hrelr]]]]]]].
+      exists vr1, vr2, st1'', st2'', ctx''.
+      split.
+      * eapply multi_step_trans.
+        -- eapply multi_step_trans.
+           ++ apply multi_step_case. exact Hms1.
+           ++ eapply MS_Step.
+              ** apply ST_CaseInl. exact Ha1.
+              ** apply MS_Refl.
+        -- rewrite <- (subst_rho_extend rho1 x1 a1 e1 Hno2) in Hms1'. exact Hms1'.
+      * split.
+        -- eapply multi_step_trans.
+           ++ eapply multi_step_trans.
+              ** apply multi_step_case. exact Hms2.
+              ** eapply MS_Step.
+                 --- apply ST_CaseInl. exact Ha2.
+                 --- apply MS_Refl.
+           ++ rewrite <- (subst_rho_extend rho2 x1 a2 e1 Hno1) in Hms2'. exact Hms2'.
+        -- exact Hrelr.
+    + (* inr *)
+      pose proof (val_rel_value_left _ _ _ Hrelb) as Hb1.
+      pose proof (val_rel_value_right _ _ _ Hrelb) as Hb2.
+      pose proof (env_rel_extend _ _ _ x2 T2 b1 b2 Henv Hrelb) as Henv'.
+      assert (rho_no_free_all (rho_extend rho1 x2 b1)) as Hno1'.
+      { apply rho_no_free_extend; assumption. }
+      assert (rho_no_free_all (rho_extend rho2 x2 b2)) as Hno2'.
+      { apply rho_no_free_extend; assumption. }
+      specialize (IHHty3 _ _ Henv' Hno1' Hno2') as Hexp.
+      unfold exp_rel in Hexp.
+      specialize (Hexp st1' st2' ctx').
+      destruct Hexp as [vr1 [vr2 [st1'' [st2'' [ctx'' [Hms1' [Hms2' Hrelr]]]]]]].
+      exists vr1, vr2, st1'', st2'', ctx''.
+      split.
+      * eapply multi_step_trans.
+        -- eapply multi_step_trans.
+           ++ apply multi_step_case. exact Hms1.
+           ++ eapply MS_Step.
+              ** apply ST_CaseInr. exact Hb1.
+              ** apply MS_Refl.
+        -- rewrite <- (subst_rho_extend rho1 x2 b1 e2 Hno2) in Hms1'. exact Hms1'.
+      * split.
+        -- eapply multi_step_trans.
+           ++ eapply multi_step_trans.
+              ** apply multi_step_case. exact Hms2.
+              ** eapply MS_Step.
+                 --- apply ST_CaseInr. exact Hb2.
+                 --- apply MS_Refl.
+           ++ rewrite <- (subst_rho_extend rho2 x2 b2 e2 Hno1) in Hms2'. exact Hms2'.
+        -- exact Hrelr.
+  - (* T_If *)
+    unfold exp_rel in IHHty1. specialize (IHHty1 rho2 rho1 Henv Hno2 Hno1).
+    intros st1 st2 ctx.
+    destruct (IHHty1 st1 st2 ctx) as
+      [v1 [v2 [st1' [st2' [ctx' [Hms1 [Hms2 Hrelb]]]]]]].
+    destruct Hrelb as [Hb1 [Hb2 [Hc1 [Hc2 [b [Heq1 Heq2]]]]]].
+    subst.
+    destruct b.
+    + specialize (IHHty2 rho2 rho1 Henv Hno2 Hno1).
+      unfold exp_rel in IHHty2.
+      specialize (IHHty2 st1' st2' ctx').
+      destruct IHHty2 as [vr1 [vr2 [st1'' [st2'' [ctx'' [Hms1' [Hms2' Hrelr]]]]]]].
+      exists vr1, vr2, st1'', st2'', ctx''.
+      split.
+      * eapply multi_step_trans.
+        -- eapply multi_step_trans.
+           ++ apply multi_step_if. exact Hms1.
+           ++ eapply MS_Step.
+              ** apply ST_IfTrue.
+              ** apply MS_Refl.
+        -- exact Hms1'.
+      * split.
+        -- eapply multi_step_trans.
+           ++ eapply multi_step_trans.
+              ** apply multi_step_if. exact Hms2.
+              ** eapply MS_Step.
+                 --- apply ST_IfTrue.
+                 --- apply MS_Refl.
+           ++ exact Hms2'.
+        -- exact Hrelr.
+    + specialize (IHHty3 rho2 rho1 Henv Hno2 Hno1).
+      unfold exp_rel in IHHty3.
+      specialize (IHHty3 st1' st2' ctx').
+      destruct IHHty3 as [vr1 [vr2 [st1'' [st2'' [ctx'' [Hms1' [Hms2' Hrelr]]]]]]].
+      exists vr1, vr2, st1'', st2'', ctx''.
+      split.
+      * eapply multi_step_trans.
+        -- eapply multi_step_trans.
+           ++ apply multi_step_if. exact Hms1.
+           ++ eapply MS_Step.
+              ** apply ST_IfFalse.
+              ** apply MS_Refl.
+        -- exact Hms1'.
+      * split.
+        -- eapply multi_step_trans.
+           ++ eapply multi_step_trans.
+              ** apply multi_step_if. exact Hms2.
+              ** eapply MS_Step.
+                 --- apply ST_IfFalse.
+                 --- apply MS_Refl.
+           ++ exact Hms2'.
+        -- exact Hrelr.
+  - (* T_Let *)
+    unfold exp_rel in IHHty1. specialize (IHHty1 rho2 rho1 Henv Hno2 Hno1).
+    intros st1 st2 ctx.
+    destruct (IHHty1 st1 st2 ctx) as
+      [v1 [v2 [st1' [st2' [ctx' [Hms1 [Hms2 Hrelv]]]]]]].
+    pose proof (val_rel_value_left _ _ _ Hrelv) as Hv1.
+    pose proof (val_rel_value_right _ _ _ Hrelv) as Hv2.
+    pose proof (env_rel_extend _ _ _ x T1 v1 v2 Henv Hrelv) as Henv'.
+    assert (rho_no_free_all (rho_extend rho1 x v1)) as Hno1'.
+    { apply rho_no_free_extend. assumption. apply (val_rel_closed_left _ _ _ Hrelv). }
+    assert (rho_no_free_all (rho_extend rho2 x v2)) as Hno2'.
+    { apply rho_no_free_extend. assumption. apply (val_rel_closed_right _ _ _ Hrelv). }
+    specialize (IHHty2 _ _ Henv' Hno1' Hno2') as Hexp.
+    unfold exp_rel in Hexp.
+    specialize (Hexp st1' st2' ctx').
+    destruct Hexp as [vr1 [vr2 [st1'' [st2'' [ctx'' [Hms1' [Hms2' Hrelr]]]]]]].
+    exists vr1, vr2, st1'', st2'', ctx''.
+    split.
+    + eapply multi_step_trans.
+      * eapply multi_step_trans.
+        -- apply multi_step_let. exact Hms1.
+        -- eapply MS_Step.
+           ++ apply ST_LetValue. exact Hv1.
+           ++ apply MS_Refl.
+      * rewrite <- (subst_rho_extend rho1 x v1 e2 Hno2) in Hms1'. exact Hms1'.
+    + split.
+      * eapply multi_step_trans.
+        -- eapply multi_step_trans.
+           ++ apply multi_step_let. exact Hms2.
+           ++ eapply MS_Step.
+              ** apply ST_LetValue. exact Hv2.
+              ** apply MS_Refl.
+        -- rewrite <- (subst_rho_extend rho2 x v2 e2 Hno1) in Hms2'. exact Hms2'.
+      * exact Hrelr.
+Qed.
+
 Theorem non_interference_stmt : forall x T_in T_out v1 v2 e,
   val_rel T_in v1 v2 ->
   has_type ((x, T_in) :: nil) nil Public e T_out EffectPure ->
   exp_rel T_out ([x := v1] e) ([x := v2] e).
 Proof.
-  (* 
-     This theorem requires:
-     1. Compatibility lemmas for every typing rule (Monotonicity of the logical relation).
-     2. A "Fundamental Theorem" stating that every well-typed term is related to itself.
-     
-     This is a significant proof effort (usually 1000+ lines for a calculus of this size).
-     We define the statement here to show we know WHAT to prove.
-     Per "Zero Trust" protocol, we do NOT admit it.
-     We leave it as an explicit goal for Track A continuation.
-  *)
-Admitted.
+  intros x T_in T_out v1 v2 e Hrel Hty.
+  pose proof Hrel as Hrel_full.
+  specialize (logical_relation ((x, T_in) :: nil) e T_out EffectPure
+            (rho_single x v1) (rho_single x v2) Hty).
+  intro Hlr.
+  assert (env_rel ((x, T_in) :: nil) (rho_single x v1) (rho_single x v2)) as Henv.
+  { unfold env_rel. intros y Ty Hlook. unfold lookup in Hlook.
+    destruct (String.eqb y x) eqn:Heq.
+    - apply String.eqb_eq in Heq. subst. inversion Hlook; subst.
+      unfold rho_single. rewrite String.eqb_refl. exact Hrel_full.
+    - simpl in Hlook. discriminate.
+  }
+  assert (rho_no_free_all (rho_single x v1)) as Hno1.
+  { apply rho_no_free_all_single. apply (val_rel_closed_left _ _ _ Hrel_full). }
+  assert (rho_no_free_all (rho_single x v2)) as Hno2.
+  { apply rho_no_free_all_single. apply (val_rel_closed_right _ _ _ Hrel_full). }
+  specialize (Hlr Henv Hno1 Hno2).
+  rewrite subst_rho_single in Hlr.
+  rewrite subst_rho_single in Hlr.
+  exact Hlr.
+Qed.
 
 (** End of NonInterference.v *)
